tests/Add.bpl
@@ -21,21 +21,26 @@ var AT#intlst: List int;
 
 function AT#Min(x:int, y: int): int { if x <= y then x else y }
 
+// -- Sequence numbering for FT ----------------------------------
+var SqnCh: <a>[Chan a][int]int;
+var SqnAct: [Actor]int;
 
 // ---------------------------------------------------------------
 // -- End of prelude ---------------------------------------------
 // ---------------------------------------------------------------
 
 procedure Add#anon$0#0()
-  modifies C, R, M, St;
+  modifies C, R, M, St, SqnCh, SqnAct;
 {
-  var IV#in1#0: int;
-  var IV#in2#0: int;
+  var in1: Chan (int);
+  var in2: Chan (int);
+  var out: Chan (int);
+  assume SqnCh[in1][0] == SqnCh[in2][0];
   assume true;
   assume true;
 }
 procedure Net#init#1()
-  modifies C, R, M, St;
+  modifies C, R, M, St, SqnCh, SqnAct;
 {
   assume C[Net#a] == 0;
   assume R[Net#a] == 0;
@@ -49,9 +54,9 @@ const unique Net#a: Chan (int);
 const unique Net#b: Chan (int);
 const unique Net#c: Chan (int);
 procedure Net#anon$1#entry#2()
-  modifies C, R, M, St;
+  modifies C, R, M, St, SqnCh, SqnAct;
 {
-  var ActionPH#y: int;
+  assume SqnAct[Net#add] == 0;
   assume L[Net#a] == (1 * Base#L);
   assume L[Net#b] == (1 * Base#L);
   assume R[Net#a] == 0;
@@ -60,6 +65,7 @@ procedure Net#anon$1#entry#2()
   assume C[Net#b] == 0;
   assume R[Net#c] == 0;
   assume C[Net#c] == 0;
+  assume (0 <= M[Net#a][0]) && (0 <= M[Net#b][0]);
   assume 0 <= R[Net#a];
   assume 0 <= C[Net#a];
   assume (R[Net#a] + C[Net#a]) <= L[Net#a];
@@ -69,16 +75,29 @@ procedure Net#anon$1#entry#2()
   assume 0 <= R[Net#c];
   assume 0 <= C[Net#c];
   assume R[Net#c] == 0;
-  assert {:msg "  Channel invariant might not hold on action entry (#9)"} R[Net#a] == (R[Net#c] + C[Net#c]);
-  assert {:msg "  Channel invariant might not hold on action entry (#10)"} R[Net#b] == (R[Net#c] + C[Net#c]);
-  assert {:msg "  Channel invariant might not hold on action entry (#11)"} (forall idx$: int :: 
+  assert {:msg "  Channel invariant might not hold on action entry (#9)"} (0 <= M[Net#a][0]) && (0 <= M[Net#b][0]);
+  assert {:msg "  Channel invariant might not hold on action entry (#10)"} R[Net#a] == (R[Net#c] + C[Net#c]);
+  assert {:msg "  Channel invariant might not hold on action entry (#11)"} R[Net#b] == (R[Net#c] + C[Net#c]);
+  assert {:msg "  Channel invariant might not hold on action entry (#12)"} (forall idx$: int :: 
     (0 <= idx$) && (idx$ < (R[Net#c] + C[Net#c])) ==> (M[Net#c][idx$] == (M[Net#a][idx$] + M[Net#b][idx$]))
+  );
+  assert {:msg "  Channel invariant might not hold on action entry (#13)"} (forall idx$: int :: 
+    (0 <= idx$) && (idx$ < (R[Net#a] + C[Net#a])) ==> (SqnCh[Net#a][idx$] == idx$)
+  );
+  assert {:msg "  Channel invariant might not hold on action entry (#14)"} (forall idx$: int :: 
+    (0 <= idx$) && (idx$ < (R[Net#b] + C[Net#b])) ==> (SqnCh[Net#b][idx$] == idx$)
+  );
+  assert {:msg "  16.3: Channel invariant might not hold on action entry (#15)"} SqnAct[Net#add] == R[Net#a];
+  assert {:msg "  17.3: Channel invariant might not hold on action entry (#16)"} (forall i: int :: 
+    (0 <= i) && (i < (R[Net#a] + C[Net#a])) ==> (SqnCh[Net#a][i] == SqnCh[Net#b][i])
+  );
+  assert {:msg "  18.3: Channel invariant might not hold on action entry (#17)"} (forall i: int :: 
+    (0 <= i) && (i < R[Net#a]) ==> (SqnCh[Net#a][i] == SqnCh[Net#c][i])
   );
 }
 procedure Net#anon$1#Add#anon$0#3()
-  modifies C, R, M, St;
+  modifies C, R, M, St, SqnCh, SqnAct;
 {
-  var ActionPH#y: int;
   var St#next: State;
   var in1#i: int;
   var in2#j: int;
@@ -93,13 +112,28 @@ procedure Net#anon$1#Add#anon$0#3()
   assume 0 <= R[Net#c];
   assume 0 <= C[Net#c];
   assume R[Net#c] == 0;
+  assume (0 <= M[Net#a][0]) && (0 <= M[Net#b][0]);
   assume R[Net#a] == (R[Net#c] + C[Net#c]);
   assume R[Net#b] == (R[Net#c] + C[Net#c]);
   assume (forall idx$: int :: 
     (0 <= idx$) && (idx$ < (R[Net#c] + C[Net#c])) ==> (M[Net#c][idx$] == (M[Net#a][idx$] + M[Net#b][idx$]))
   );
+  assume (forall idx$: int :: 
+    (0 <= idx$) && (idx$ < (R[Net#a] + C[Net#a])) ==> (SqnCh[Net#a][idx$] == idx$)
+  );
+  assume (forall idx$: int :: 
+    (0 <= idx$) && (idx$ < (R[Net#b] + C[Net#b])) ==> (SqnCh[Net#b][idx$] == idx$)
+  );
+  assume SqnAct[Net#add] == R[Net#a];
+  assume (forall i: int :: 
+    (0 <= i) && (i < (R[Net#a] + C[Net#a])) ==> (SqnCh[Net#a][i] == SqnCh[Net#b][i])
+  );
+  assume (forall i: int :: 
+    (0 <= i) && (i < R[Net#a]) ==> (SqnCh[Net#a][i] == SqnCh[Net#c][i])
+  );
   assume true;
   assume (1 <= C[Net#a]) && (1 <= C[Net#b]);
+  assert {:msg "  4.14: Precondition might not hold for instance at 21.5"} SqnCh[Net#a][R[Net#a] - 0] == SqnCh[Net#b][R[Net#b] - 0];
   in1#i := M[Net#a][R[Net#a]];
   R[Net#a] := R[Net#a] + 1;
   C[Net#a] := C[Net#a] - 1;
@@ -107,7 +141,9 @@ procedure Net#anon$1#Add#anon$0#3()
   R[Net#b] := R[Net#b] + 1;
   C[Net#b] := C[Net#b] - 1;
   M[Net#c][R[Net#c] + C[Net#c]] := in1#i + in2#j;
+  SqnCh[Net#c][R[Net#c] + C[Net#c]] := SqnAct[Net#add];
   C[Net#c] := C[Net#c] + 1;
+  SqnAct[Net#add] := SqnAct[Net#add] + 1;
   assume 0 <= R[Net#a];
   assume 0 <= C[Net#a];
   assume (R[Net#a] + C[Net#a]) <= L[Net#a];
@@ -117,16 +153,29 @@ procedure Net#anon$1#Add#anon$0#3()
   assume 0 <= R[Net#c];
   assume 0 <= C[Net#c];
   assume R[Net#c] == 0;
-  assert {:msg "  Action at 3.3 ('anon$0') for actor instance 'add' might not preserve the channel invariant (#21)"} R[Net#a] == (R[Net#c] + C[Net#c]);
-  assert {:msg "  Action at 3.3 ('anon$0') for actor instance 'add' might not preserve the channel invariant (#22)"} R[Net#b] == (R[Net#c] + C[Net#c]);
-  assert {:msg "  Action at 3.3 ('anon$0') for actor instance 'add' might not preserve the channel invariant (#23)"} (forall idx$: int :: 
+  assert {:msg "  Action at 3.3 ('anon$0') for actor instance 'add' might not preserve the channel invariant (#27)"} (0 <= M[Net#a][0]) && (0 <= M[Net#b][0]);
+  assert {:msg "  Action at 3.3 ('anon$0') for actor instance 'add' might not preserve the channel invariant (#28)"} R[Net#a] == (R[Net#c] + C[Net#c]);
+  assert {:msg "  Action at 3.3 ('anon$0') for actor instance 'add' might not preserve the channel invariant (#29)"} R[Net#b] == (R[Net#c] + C[Net#c]);
+  assert {:msg "  Action at 3.3 ('anon$0') for actor instance 'add' might not preserve the channel invariant (#30)"} (forall idx$: int :: 
     (0 <= idx$) && (idx$ < (R[Net#c] + C[Net#c])) ==> (M[Net#c][idx$] == (M[Net#a][idx$] + M[Net#b][idx$]))
+  );
+  assert {:msg "  Action at 3.3 ('anon$0') for actor instance 'add' might not preserve the channel invariant (#31)"} (forall idx$: int :: 
+    (0 <= idx$) && (idx$ < (R[Net#a] + C[Net#a])) ==> (SqnCh[Net#a][idx$] == idx$)
+  );
+  assert {:msg "  Action at 3.3 ('anon$0') for actor instance 'add' might not preserve the channel invariant (#32)"} (forall idx$: int :: 
+    (0 <= idx$) && (idx$ < (R[Net#b] + C[Net#b])) ==> (SqnCh[Net#b][idx$] == idx$)
+  );
+  assert {:msg "  16.3: Action at 3.3 ('anon$0') for actor instance 'add' might not preserve the channel invariant (#33)"} SqnAct[Net#add] == R[Net#a];
+  assert {:msg "  17.3: Action at 3.3 ('anon$0') for actor instance 'add' might not preserve the channel invariant (#34)"} (forall i: int :: 
+    (0 <= i) && (i < (R[Net#a] + C[Net#a])) ==> (SqnCh[Net#a][i] == SqnCh[Net#b][i])
+  );
+  assert {:msg "  18.3: Action at 3.3 ('anon$0') for actor instance 'add' might not preserve the channel invariant (#35)"} (forall i: int :: 
+    (0 <= i) && (i < R[Net#a]) ==> (SqnCh[Net#a][i] == SqnCh[Net#c][i])
   );
 }
 procedure Net#anon$1#exit#4()
-  modifies C, R, M, St;
+  modifies C, R, M, St, SqnCh, SqnAct;
 {
-  var ActionPH#y: int;
   assume L[Net#a] == (1 * Base#L);
   assume L[Net#b] == (1 * Base#L);
   assume 0 <= R[Net#a];
@@ -138,19 +187,33 @@ procedure Net#anon$1#exit#4()
   assume 0 <= R[Net#c];
   assume 0 <= C[Net#c];
   assume R[Net#c] == 0;
+  assume (0 <= M[Net#a][0]) && (0 <= M[Net#b][0]);
   assume R[Net#a] == (R[Net#c] + C[Net#c]);
   assume R[Net#b] == (R[Net#c] + C[Net#c]);
   assume (forall idx$: int :: 
     (0 <= idx$) && (idx$ < (R[Net#c] + C[Net#c])) ==> (M[Net#c][idx$] == (M[Net#a][idx$] + M[Net#b][idx$]))
   );
+  assume (forall idx$: int :: 
+    (0 <= idx$) && (idx$ < (R[Net#a] + C[Net#a])) ==> (SqnCh[Net#a][idx$] == idx$)
+  );
+  assume (forall idx$: int :: 
+    (0 <= idx$) && (idx$ < (R[Net#b] + C[Net#b])) ==> (SqnCh[Net#b][idx$] == idx$)
+  );
+  assume SqnAct[Net#add] == R[Net#a];
+  assume (forall i: int :: 
+    (0 <= i) && (i < (R[Net#a] + C[Net#a])) ==> (SqnCh[Net#a][i] == SqnCh[Net#b][i])
+  );
+  assume (forall i: int :: 
+    (0 <= i) && (i < R[Net#a]) ==> (SqnCh[Net#a][i] == SqnCh[Net#c][i])
+  );
   assume !((R[Net#a] + C[Net#a]) < L[Net#a]);
   assume !((R[Net#b] + C[Net#b]) < L[Net#b]);
   assume !((1 <= C[Net#a]) && (1 <= C[Net#b]));
-  ActionPH#y := M[Net#c][0];
-  assert {:msg "  9.13: Network action postcondition might not hold"} ActionPH#y == (M[Net#a][0] + M[Net#b][0]);
+  assert {:msg "  12.13: Network action postcondition might not hold"} M[Net#c][0] == (M[Net#a][0] + M[Net#b][0]);
+  assert {:msg "  13.13: Network action postcondition might not hold"} SqnCh[Net#c][0] == 0;
   R[Net#c] := R[Net#c] + C[Net#c];
   C[Net#c] := C[Net#c] - (1 * Base#L);
-  assert {:msg "  8.3: The network might leave unread tokens on channel a"} C[Net#a] == 0;
-  assert {:msg "  8.3: The network might leave unread tokens on channel b"} C[Net#b] == 0;
-  assert {:msg "  8.3: The network might not produce the specified number of tokens on output out"} C[Net#c] == 0;
+  assert {:msg "  10.3: The network might leave unread tokens on channel a"} C[Net#a] == 0;
+  assert {:msg "  10.3: The network might leave unread tokens on channel b"} C[Net#b] == 0;
+  assert {:msg "  10.3: The network might not produce the specified number of tokens on output out"} C[Net#c] == 0;
 }
